Add Monad laws to Monad class

Classes/Monad.v
@@ -1,15 +1,44 @@
+Require Import Classes.Applicative.
 
-Class Monad (M : Type -> Type) : Type :=
+Class Monad (M : Type -> Type) `{Applicative M} : Type :=
 {
-  returnM : forall A, A -> M A;
-  bindM : forall A B, M A  -> (A -> M B) -> M B;
+  bindM : forall {A B}, M A  -> (A -> M B) -> M B;
+  bind_id_left : forall (A B : Type) (f : A -> M B) (a : A), 
+    bindM (pure a) f = f a;
+  bind_id_right : forall (A : Type) (MA : M A),
+    bindM MA pure = MA;
+  bind_assoc : forall (A B C : Type) (MA : M A) (f : A -> M B) (g : B -> M C),
+    bindM (bindM MA f) g = bindM MA (fun a => bindM (f a) g);
 }.
-Arguments Build_Monad {_ _ _}.
-Arguments returnM {_ _ _}.
-Arguments bindM {_ _ _ _}.
+
+Arguments Build_Monad {_ _ _ _}.
+Arguments bindM {_ _ _ _ _ _}.
+
+Lemma bind_equiv_l {M : Type -> Type} {A B : Type} `{Monad M} : 
+  forall (m m' : M A) k,
+  m = m' -> bindM m k = @bindM M _ _ _ A B m' k.
+Proof.
+  intros. rewrite H2. reflexivity.
+Qed.
+
+Lemma bind_equiv_r {M : Type -> Type} {A B : Type} `{Monad M} : 
+  forall (m : M A) k k',
+  k = k' -> bindM m k = @bindM M _ _ _ A B m k'.
+Proof.
+  intros. rewrite H2. reflexivity.
+Qed.
 
 Notation "x '<<' y ; z" := (bindM y (fun x => z))
   (at level 20, y at level 100, z at level 200, only parsing).
 
 Notation "x ;; z" := (bindM x (fun _ => z))
     (at level 100, z at level 200, only parsing, right associativity).
+
+Section MonadTransformer.
+  Context {M} `{Monad M}.
+
+  Class MonadT (T : (Type -> Type) -> Type -> Type) : Type :=
+  {
+    liftT : forall {A}, M A -> T M A;
+  }.
+End MonadTransformer.
